
**1.0)** Take the vectors $\textbf{i}$ and $\textbf{j}$. In an associativity test, we have the following table:

| Step | Expression                                     | Result        |
| ---- | ---------------------------------------------- | ------------- |
| 1    | $(\textbf{i}\times\textbf{i})$                 | $\textbf{0}$  |
| 1    | $(\textbf{i}\times\textbf{j})$                 | $\textbf{k}$  |
| 2    | $(\textbf{i}\times\textbf{i})\times\textbf{j}$ | $\textbf{0}$  |
| 2    | $\textbf{i}\times(\textbf{i}\times\textbf{j})$ | $-\textbf{k}$ |

Therefore, $(\textbf{i}\times\textbf{i})\times\textbf{j}\neq\textbf{i}\times(\textbf{i}\times\textbf{j})$. 


**1.1)** These statements are equivalent to $1<\epsilon k$, where $k\in \{n,\;n^2,\sqrt{n}\}$. Since $1$ and $\epsilon$ are members of Archimedian Ordered Fields, **(a)** is true straightforwardly from the Archimedian property. Then 
$$\begin{align*}

&1<\epsilon n<\epsilon n^2\\
\implies &1<\epsilon n^2\text{,}
\end{align*}$$
which demonstrates **(b)**. 

Suppose that $n$ can take any value in the set of perfect squares; then $\sqrt{n}$ can take any value in $\mathbb{N}$. Therefore, **(c)** is equivalent to **(a)**, which we know is true. 


**1.4)** It is the case by the additive inverse property that something equal to $-a$ iff adding it to $a$ gives the additive identity. By the distributive property of the real numbers,
$$(-1)a+a=a(-1+1)\text{,}$$
which is equal to $0$; this is what we want. 


**1.5)** Let $b=a^{-1}$, and suppose that there existed some other inverse $c$ of $a$.  Then $ab=1$ and $ac=1$, so $ab=ac$, which is the case iff $bab=bac$, which is the case iff $b=c$; therefore $b=a^{-1}$ is unique.


**1.6)** Use the definition of the function:
$$|x|=\begin{cases}x&\text{if }x\geq 0\\ -x&\text{if }x<0\text{,}\end{cases}$$
which can be applied to $a$ and $b$. We can directly
$$|ab|=\begin{cases}ab&\text{if }ab\geq 0\\-ab&\text{if }ab<0\text{,}\end{cases}$$
But taking the function around $a$ and $b$ individually gives four cases:

| Case | Inequality 1.1 | Inequality 1.2 | Inequality 2 | Function Value |
| ---- | -------------- | -------------- | ------------ | -------------- |
| 1    | $a\geq 0$      | $b\geq 0$      | $ab\geq 0$   | $ab$           |
| 2    | $a\geq 0$      | $b<0$          | $ab<0$       | $-ab$          |
| 3    | $a<0$          | $b\geq 0$      | $ab<0$       | $-ab$          |
| 4    | $a<0$          | $b<0$          | $ab\geq 0$   | $ab$           |
Tying together:
$$|a||b|=\begin{cases}ab&\text{if }ab\geq 0\\-ab&\text{if }ab<0\text{.}\end{cases}$$

**1.8)** By the basic properties of the absolute value, we know that 
$$|a-c|\leq |a-b|-|c-b|\text{.}$$
Now, it's also straightforward that 
$$|a-b|-|c-b|\leq|a-b|+|c-b|\text{.}$$
Next, take the fact that $|a-b|<\delta$ and $|a-c|<\delta$ implies that
$$|a-b|+|c-b|<2\delta\text{.}$$
These three inequalities, in fact, establish that 
$$|a-c|\leq |a-b|-|c-b|\leq|a-b|+|c-b|<2\delta\text{,}$$
which implies that $|a-c|<2\delta$. Hence we only need to choose some $\delta$ such that $2\delta<\epsilon$, such as $\frac{\epsilon}{4}$, to satisfy our needs. 

**1.10)** If $$\begin{pmatrix}a&b&c&d\end{pmatrix}=\begin{pmatrix}1&2&1&2\end{pmatrix}\text{,}$$ then $a-c=0$ and $b-d=0$. If 
$$\begin{pmatrix}a&b&c&d\end{pmatrix}=\begin{pmatrix}2&1&2&1\end{pmatrix}\text{,}$$ then $a+c=4$ and $b+d=2$. Then by the Law of Trichotomy, neither the statement in **(a)** nor the statement in 

**1.11)**

