
**1.03)** By the axiom of additive identity, our expression is equal to zero iff adding it to any $a$ gives $a$. Now for an arbitrary $a$,
$$a+a0=a1+a0\text{,}$$
by the axiom of multiplicative identity. Then
$$a1+a0=a(1+0)\text{,}$$
by the axiom of distributivity. Then 
$$a(1+0)=a1\text{,}$$
by the law of additive identity. Then
$$a1=a\text{,}$$
by the law of multiplicative identity. So, it is demonstrated that
$$a+a0=a\text{,}$$
and as a result demonstrated that 
$$a0=0$$
for any arbitrary $a$, as required.

By the axiom of the additive inverse, $(-1)(-1)=1$ iff $(-1)(-1)-1=0$. By the axiom of distributivity,
$$(-1)(-1)-1=(-1)(-1+1)\text{,}$$
and by the axioms of additive commutativity and the additive inverse, 
 $$(-1)(-1+1)=(-1)0\text{.}$$
Then by the first statement proven,
$$(-1)0=0\text{.}$$
So, it is demonstrated that $(-1)(-1)-1=0$, which is the case iff $(-1)(-1)=1$, so our desired statement is proven.


**1.07)** For all $a$, $b$, and $c$ in $\mathbb{R}$, we know that $a-b$ and $b-c$ are in $\mathbb{R}$. Now, we can apply the triangle to both $a-b$ and $b-c$, as they are both real numbers. Start with
$$|a-c|=|(a-b)+(b-c)|\text{.}$$
Then, by the triangle inequality, 
$$|(a-b)+(b-c)|\leq|a-b|+|b-c|\text{,}$$
So, we have
$$|a-c|\leq |a-b|+|b-c|\text{,}$$
which was to be demonstrated.