Ah, let me try a different approach using divisibility properties.

If $2 = x^2-2y^2$, then:
1. $2 \mid x^2-2y^2$
2. Therefore $x^2 \equiv 2y^2 \pmod{2}$
3. The LHS must be even (as 2 divides RHS)
4. So $x$ must be even, say $x = 2k$
5. Substituting: $2 = 4k^2-2y^2$
6. Divide by 2: $1 = 2k^2-y^2$
7. Therefore $2k^2 = 1+y^2$
8. So $2 \mid (1+y^2)$
9. But this is impossible because...

Actually, I'm stuck. I can see from step 8 that $y$ must be odd, but I'm not seeing how to reach a clear contradiction using divisibility. Could you help point me in the right direction?